more

src/Iris/Examples/Exp.lean
@@ -11,6 +11,14 @@ open BI
 
 variable {u} [BI.{u} PROP]
 
+inductive Binder where
+| anon : Binder
+| str : String → Binder
+deriving Inhabited, BEq, Repr
+
+instance : Coe String Binder where
+  coe := Binder.str
+
 def Loc : Type := Nat
 
 inductive Binop where
@@ -20,12 +28,13 @@ mutual
 inductive Val where
 | nat : Nat -> Val
 | loc : Loc -> Val
-| recv : String -> String -> Exp -> Val
+| recv : Binder -> Binder -> Exp -> Val
 inductive Exp where
 | val : Val -> Exp
 | var : String -> Exp
 | binop : Exp -> Binop -> Exp -> Exp
-| rece : String -> String -> Exp -> Exp
+| rece : Binder -> Binder -> Exp -> Exp
+| lete : Binder -> Exp -> Exp -> Exp
 | app : Exp -> Exp -> Exp
 | ife : Exp -> Exp -> Exp -> Exp
 end
@@ -34,9 +43,15 @@ def subst (x : String) (v : Val) : Exp → Exp
   | .val v => .val v
   | .var y => if x == y then .val v else .var y
   | .binop e1 o e2 => .binop (subst x v e1) o (subst x v e2)
-  | .rece f y e' => .rece f y (if x == f || x == y then e' else subst x v e')
+  | .rece f y e' => .rece f y (if .str x == f || .str x == y then e' else subst x v e')
+  | .lete y e1 e2 => .lete y (subst x v e1) (if .str x == y then e2 else subst x v e2)
   | .app e1 e2 => .app (subst x v e1) (subst x v e2)
   | .ife e1 e2 e3 => .ife (subst x v e1) (subst x v e2)  (subst x v e3)
+
+def subst' (x : Binder) (v : Val) (e : Exp) : Exp :=
+  match x with
+  | .anon => e
+  | .str x => subst x v e
 
 def wp [BI PROP] (e : Exp) (P : Val -> PROP) : PROP := by sorry
 
@@ -50,21 +65,37 @@ inductive Exp where
 | val : Expr -> Exp -- we do not need to reify values
 | var : String -> Exp
 | binop : Exp -> Expr -> Exp -> Exp
-| rece : String -> String -> Exp -> Exp
+| rece : Binder -> Binder -> Exp -> Exp
+| lete : Binder -> Exp -> Exp -> Exp
 | app : Exp -> Exp -> Exp
 | ife : Exp -> Exp -> Exp -> Exp
 | unk : Expr -> Exp
 deriving Inhabited, Repr
+
+def Binder.unreify (b : Binder) : Expr :=
+  match b with
+  | Binder.anon => mkConst ``Binder.anon
+  | Binder.str s => mkApp (mkConst ``Binder.str) (mkStrLit s)
 
 -- should this be ToExpr?
 def Exp.unreify : Exp → Expr
   | .val v => mkApp (mkConst ``Lang.Exp.val) v
   | .var v => mkApp (mkConst ``Lang.Exp.var) (mkStrLit v)
   | .binop e1 o e2 => mkApp3 (mkConst ``Lang.Exp.binop) (unreify e1) o (unreify e2)
-  | .rece f x e => mkApp3 (mkConst ``Lang.Exp.rece) (mkStrLit f) (mkStrLit x) (unreify e)
+  | .rece f x e => mkApp3 (mkConst ``Lang.Exp.rece) (Binder.unreify f) (Binder.unreify x) (unreify e)
+  | .lete x e1 e2 => mkApp3 (mkConst ``Lang.Exp.lete) (Binder.unreify x) (unreify e1) (unreify e2)
   | .app e1 e2 => mkApp2 (mkConst ``Lang.Exp.app) (unreify e1) (unreify e2)
   | .ife e1 e2 e3 => mkApp3 (mkConst ``Lang.Exp.ife) (unreify e1) (unreify e2) (unreify e3)
   | .unk e => e
+
+def Binder.reify (e : Expr) : Option Binder :=
+  match_expr e with
+  | Binder.anon => some (.anon)
+  | Binder.str s =>
+    match s with
+    | .lit (.strVal v) => some (.str v)
+    | _ => none
+  | _ => none
 
 partial def reify (e : Expr) : Exp :=
   match_expr e with
@@ -75,9 +106,13 @@ partial def reify (e : Expr) : Exp :=
     | _ => .unk e
   | Lang.Exp.binop e1 o e2 => .binop (reify e1) o (reify e2)
   | Lang.Exp.rece f x e' =>
-    match f, x with
-    | .lit (.strVal f), .lit (.strVal x) => .rece f x (reify e')
-    | _, _ => .unk e'
+    match Binder.reify f, Binder.reify x with
+    | some f, some x => .rece f x (reify e')
+    | _, _ => .unk e
+  | Lang.Exp.lete x e1 e2 =>
+    match Binder.reify x with
+    | some x => .lete x (reify e1) (reify e2)
+    | _ => .unk e
   | Lang.Exp.app e1 e2 => .app (reify e1) (reify e2)
   | Lang.Exp.ife e1 e2 e3 => .ife (reify e1) (reify e2) (reify e3)
   | _ => .unk e
@@ -87,10 +122,16 @@ def subst (x : String) (v : Expr) (e : Exp) : Exp :=
   | .val _ => e
   | .var y => if x == y then .val v else e
   | .binop e1 o e2 => .binop (subst x v e1) o (subst x v e2)
-  | .rece f y e' => .rece f y (if x == f || x == y then e' else subst x v e')
+  | .rece f y e' => .rece f y (if .str x == f || .str x == y then e' else subst x v e')
+  | .lete y e1 e2 => .lete y (subst x v e1) (if .str x == y then e2 else subst x v e2)
   | .app e1 e2 => .app (subst x v e1) (subst x v e2)
   | .ife e1 e2 e3 => .ife (subst x v e1) (subst x v e2)  (subst x v e3)
   | .unk e => .unk (mkApp3 (mkConst ``Lang.subst) (mkStrLit x) v e)
+
+def subst' (x : Binder) (v : Expr) (e : Exp) : Exp :=
+  match x with
+  | .anon => e
+  | .str x => subst x v e
 
 end Reify
 
